Stop using Iris abstract languages.

theories/zoo/language/language.v
@@ -1,9 +1,5 @@
 From zoo Require Import
   prelude.
-From zoo.iris.program_logic Require Export
-  language
-  ectx_language
-  ectxi_language.
 From zoo.language Require Export
   semantics.
 From zoo Require Import
@@ -12,31 +8,432 @@ From zoo Require Import
 Implicit Types e : expr.
 Implicit Types es : list expr.
 Implicit Types v : val.
-Implicit Types K : ectx.
 Implicit Types σ : state.
-Implicit Types κ : list observation.
+Implicit Types κ κs : list observation.
+Implicit Types k : ectxi.
+Implicit Types K : ectx.
+Implicit Types ρ : config.
 
-Lemma zoo_mixin :
-  EctxiLanguageMixin of_val to_val ectxi_fill base_step.
+Declare Scope expr_scope.
+Delimit Scope expr_scope with E.
+Bind Scope expr_scope with expr.
+
+Declare Scope val_scope.
+Delimit Scope val_scope with V.
+Bind Scope val_scope with val.
+
+Class AsVal e v :=
+  as_val : of_val v = e.
+
+Inductive prim_step tid e1 σ1 κ e2 σ2 es : Prop :=
+  | base_step_fill_prim_step' K e1' e2' :
+      e1 = fill K e1' →
+      e2 = fill K e2' →
+      base_step tid e1' σ1 κ e2' σ2 es →
+      prim_step tid e1 σ1 κ e2 σ2 es.
+#[global] Arguments base_step_fill_prim_step' {_ _ _ _ _ _ _}.
+
+Definition step ρ1 κ ρ2 :=
+  ∃ tid e1 e2 σ2 es,
+  prim_step tid e1 ρ1.2 κ e2 σ2 es ∧
+  ρ1.1 !! tid = Some e1 ∧
+  ρ2 = (<[tid := e2]> ρ1.1 ++ es, σ2).
+
+Inductive nsteps : nat → config → list observation → config → Prop :=
+  | nsteps_refl ρ :
+     nsteps 0 ρ [] ρ
+  | nsteps_l n ρ1 ρ2 ρ3 κ κs :
+     step ρ1 κ ρ2 →
+     nsteps n ρ2 κs ρ3 →
+     nsteps (S n) ρ1 (κ ++ κs) ρ3.
+#[local] Hint Constructors nsteps : core.
+
+Definition silent_step ρ1 ρ2 :=
+  ∃ κ,
+  step ρ1 κ ρ2.
+
+Definition base_reducible tid e σ :=
+  ∃ κ e' σ' es,
+  base_step tid e σ κ e' σ' es.
+Definition base_reducible_no_obs tid e σ :=
+  ∃ e' σ' es,
+  base_step tid e σ [] e' σ' es.
+Definition base_irreducible tid e σ :=
+  ∀ κ e' σ' es,
+  ¬ base_step tid e σ κ e' σ' es.
+Definition base_stuck tid e σ :=
+  to_val e = None ∧
+  base_irreducible tid e σ.
+Definition base_atomic e :=
+  ∀ tid σ κ e' σ' es,
+  base_step tid e σ κ e' σ' es →
+  is_Some (to_val e').
+
+Record pure_base_step e1 e2 := {
+  pure_base_step_safe tid σ1 :
+    base_reducible_no_obs tid e1 σ1 ;
+  pure_base_step_det tid σ1 κ e2' σ2 es :
+    base_step tid e1 σ1 κ e2' σ2 es →
+      κ = [] ∧
+      σ2 = σ1 ∧
+      e2' = e2 ∧
+      es = [] ;
+}.
+
+Definition reducible tid e σ :=
+  ∃ κ e' σ' es,
+  prim_step tid e σ κ e' σ' es.
+Definition reducible_no_obs tid e σ :=
+  ∃ e' σ' es,
+  prim_step tid e σ [] e' σ' es.
+Definition irreducible tid e σ :=
+  ∀ κ e' σ' es,
+  ¬ prim_step tid e σ κ e' σ' es.
+Definition stuck tid e σ :=
+  to_val e = None ∧
+  irreducible tid e σ.
+Definition not_stuck tid e σ :=
+  is_Some (to_val e) ∨
+  reducible tid e σ.
+Class Atomic e :=
+  atomic tid σ e' κ σ' es :
+    prim_step tid e σ κ e' σ' es →
+    is_Some (to_val e').
+Definition safe ρ :=
+  ∀ ρ',
+  rtc silent_step ρ ρ' →
+  Foralli (λ tid e, not_stuck tid e ρ'.2) ρ'.1.
+
+Record pure_step e1 e2 := {
+  pure_step_safe tid σ1 :
+    reducible_no_obs tid e1 σ1 ;
+  pure_step_det tid σ1 κ e2' σ2 es :
+    prim_step tid e1 σ1 κ e2' σ2 es →
+      κ = [] ∧
+      σ2 = σ1 ∧
+      e2' = e2 ∧
+      es = [] ;
+}.
+
+Class Context (K : expr → expr) := {
+  context_fill_not_val e :
+    to_val e = None →
+    to_val (K e) = None ;
+  context_fill_step tid e1 σ1 κ e2 σ2 es :
+    prim_step tid e1 σ1 κ e2 σ2 es →
+    prim_step tid (K e1) σ1 κ (K e2) σ2 es ;
+  context_fill_step_inv tid e1' σ1 κ e2 σ2 es :
+    to_val e1' = None →
+    prim_step tid (K e1') σ1 κ e2 σ2 es →
+      ∃ e2',
+      e2 = K e2' ∧
+      prim_step tid e1' σ1 κ e2' σ2 es ;
+}.
+
+Class PureExec (ϕ : Prop) n e1 e2 :=
+  pure_exec :
+    ϕ →
+    relations.nsteps pure_step n e1 e2.
+
+Definition sub_redexes_are_values e :=
+  ∀ K e', e = fill K e' →
+  to_val e' = None →
+  K = [].
+
+#[global] Instance filli_inj k :
+  Inj (=) (=) (filli k).
 Proof.
-  split.
-  all: try apply _.
-  all: eauto using
-    to_of_val,
-    of_to_val,
-    val_base_stuck,
-    ectxi_fill_val,
-    ectxi_fill_no_val_inj,
-    base_step_ectxi_fill_val.
+  induction k; intros ?*; naive_solver.
+Qed.
+Lemma filli_val k e :
+  is_Some (to_val (filli k e)) →
+  is_Some (to_val e).
+Proof.
+  intros (v & ?). destruct k; done.
+Qed.
+Lemma filli_no_val_inj k1 e1 k2 e2 :
+  to_val e1 = None →
+  to_val e2 = None →
+  filli k1 e1 = filli k2 e2 →
+  k1 = k2.
+Proof.
+  move: k1.
+  induction k2; intros k1; destruct k1; try naive_solver.
+  intros H1 H2 [= -> -> H%app_inj_2]; first naive_solver.
+  simpl. do 3 f_equal.
+  apply (f_equal reverse) in H.
+  rewrite !reverse_app !reverse_cons -!fmap_reverse /= in H.
+  match goal with |- ?vs1 = ?vs2 =>
+    apply (inj reverse);
+    remember (reverse vs1) as vs1';
+    remember (reverse vs2) as vs2';
+    clear- H1 H2 H; move: vs2' H; induction vs1'; intros []; naive_solver
+  end.
+Qed.
+Lemma base_step_filli_val tid k e σ1 κ e2 σ2 es :
+  base_step tid (filli k e) σ1 κ e2 σ2 es →
+  is_Some (to_val e).
+Proof.
+  move: κ e2.
+  induction k; try (inversion_clear 1; eauto || done).
+  all: inversion_clear 1.
+  all:
+    match goal with H: _ ++ _ :: of_vals ?vs1 = of_vals ?vs2 |- _ =>
+      apply (f_equal reverse) in H;
+      rewrite reverse_app reverse_cons -!fmap_reverse /= in H;
+      remember (reverse vs1) as vs1';
+      remember (reverse vs2) as vs2';
+      clear- H; move: vs2' H; induction vs1'; intros []; naive_solver
+    end.
 Qed.
 
-Canonical zoo_ectxi_lang :=
-  Build_ectxi_language zoo_mixin.
-Canonical zoo_ectx_lang :=
-  EctxLanguageOfEctxi zoo_ectxi_lang.
-Canonical zoo :=
-  LanguageOfEctx zoo_ectx_lang.
-#[global] Arguments zoo : simpl never.
+#[global] Instance fill_inj K :
+  Inj (=) (=) (fill K).
+Proof.
+  induction K as [| k K IH].
+  all: rewrite /Inj.
+  all: naive_solver.
+Qed.
+Lemma fill_nil e :
+  fill [] e = e.
+Proof.
+  done.
+Qed.
+Lemma fill_app K1 K2 e :
+  fill (K1 ++ K2) e = fill K2 (fill K1 e).
+Proof.
+  apply foldl_app.
+Qed.
+Lemma fill_val K e :
+  is_Some (to_val (fill K e)) →
+  is_Some (to_val e).
+Proof.
+  move: e. induction K as [| k K IH] => e //=.
+  intros ?%IH%filli_val => //.
+Qed.
+Lemma fill_not_val K e :
+  to_val e = None →
+  to_val (fill K e) = None.
+Proof.
+  rewrite !eq_None_not_Some.
+  eauto using fill_val.
+Qed.
+
+Lemma base_step_not_val tid e1 σ1 κ e2 σ2 es :
+  base_step tid e1 σ1 κ e2 σ2 es →
+  to_val e1 = None.
+Proof.
+  destruct 1; naive_solver.
+Qed.
+Lemma step_by_val tid K1 K2 e1 e2 σ1 κ e2' σ2 es :
+  fill K1 e1 = fill K2 e2 →
+  to_val e1 = None →
+  base_step tid e2 σ1 κ e2' σ2 es →
+    ∃ K,
+    K2 = K ++ K1.
+Proof.
+  intros Hfill Hred Hstep.
+  move: K2 Hfill. induction K1 as [| k1 K1 IH] using rev_ind => /= K2 Hfill.
+  - eauto using app_nil_r.
+  - destruct K2 as [| k2 K2 _] using rev_ind; simplify_eq/=.
+    { rewrite fill_app in Hstep. apply base_step_filli_val in Hstep.
+      apply fill_val in Hstep. apply not_eq_None_Some in Hstep. done.
+    }
+    rewrite !fill_app /= in Hfill.
+    assert (k1 = k2) as ->.
+    { eapply filli_no_val_inj, Hfill.
+      all: eauto using fill_not_val, base_step_not_val.
+    }
+    simplify_eq. destruct (IH K2) as [K ->]; auto.
+    exists K. rewrite assoc //.
+Qed.
+Lemma base_step_fill_val tid K e σ1 κ e2 σ2 es :
+  base_step tid (fill K e) σ1 κ e2 σ2 es →
+    is_Some (to_val e) ∨
+    K = [].
+Proof.
+  destruct K as [| k K _] using rev_ind; simpl; first by auto.
+  rewrite fill_app /=. intros ?%base_step_filli_val.
+  eauto using fill_val.
+Qed.
+
+Lemma base_reducible_no_obs_base_reducible tid e σ :
+  base_reducible_no_obs tid e σ →
+  base_reducible tid e σ.
+Proof.
+  intros (? & ? & ? & ?). eexists. eauto.
+Qed.
+
+Lemma base_step_prim_step tid e1 σ1 κ e2 σ2 es :
+  base_step tid e1 σ1 κ e2 σ2 es →
+  prim_step tid e1 σ1 κ e2 σ2 es.
+Proof.
+  apply (base_step_fill_prim_step' []).
+  all: rewrite ?fill_nil //.
+Qed.
+Lemma prim_step_not_val tid e σ κ e' σ' es :
+  prim_step tid e σ κ e' σ' es →
+  to_val e = None.
+Proof.
+  intros [? ? ? -> -> ?%base_step_not_val].
+  apply eq_None_not_Some. intros ?%fill_val%eq_None_not_Some; done.
+Qed.
+Lemma reducible_not_val tid e σ :
+  reducible tid e σ →
+  to_val e = None.
+Proof.
+  intros (? & ? & ? & ? & ?).
+  eauto using prim_step_not_val.
+Qed.
+Lemma reducible_no_obs_reducible tid e σ :
+  reducible_no_obs tid e σ →
+  reducible tid e σ.
+Proof.
+  intros (? & ? & ? & ?).
+  eexists. eauto.
+Qed.
+Lemma base_reducible_reducible tid e σ :
+  base_reducible tid e σ →
+  reducible tid e σ.
+Proof.
+  intros (κ & e' & σ' & es & ?).
+  exists κ, e', σ', es.
+  apply base_step_prim_step. done.
+Qed.
+
+Lemma base_atomic_atomic e :
+  base_atomic e →
+  sub_redexes_are_values e →
+  Atomic e.
+Proof.
+  intros Hatomic_step Hatomic_fill tid σ κ e' σ' es [K e1' e2' -> -> Hstep].
+  assert (K = []) as -> by eauto 10 using base_step_not_val.
+  rewrite fill_nil. eapply Hatomic_step. rewrite fill_nil //.
+Qed.
+
+Lemma base_reducible_fill_prim_step tid K e1 σ1 κ e2 σ2 es :
+  base_reducible tid e1 σ1 →
+  prim_step tid (fill K e1) σ1 κ e2 σ2 es →
+    ∃ e2',
+    e2 = fill K e2' ∧
+    base_step tid e1 σ1 κ e2' σ2 es.
+Proof.
+  intros (κ' & e2'' & σ2'' & es'' & HhstepK) [K' e1' e2' HKe1 -> Hstep].
+  edestruct (step_by_val tid K) as [K'' ?]; eauto using base_step_not_val; simplify_eq/=.
+  rewrite fill_app in HKe1; simplify_eq.
+  exists (fill K'' e2'). rewrite fill_app; split; first done.
+  apply base_step_fill_val in HhstepK as [[v ?] | ?]; simplify_eq.
+  { apply base_step_not_val in Hstep. simplify_eq. }
+  rewrite !fill_nil //.
+Qed.
+Lemma base_reducible_prim_step tid e1 σ1 κ e2 σ2 es :
+  base_reducible tid e1 σ1 →
+  prim_step tid e1 σ1 κ e2 σ2 es →
+  base_step tid e1 σ1 κ e2 σ2 es.
+Proof.
+  intros.
+  edestruct (base_reducible_fill_prim_step tid []) as (? & ? & ?).
+  all: rewrite ?fill_nil; eauto.
+  simplify. done.
+Qed.
+
+Lemma pure_base_step_pure_step e1 e2 :
+  pure_base_step e1 e2 →
+  pure_step e1 e2.
+Proof.
+  intros [Hsafe Hdet]. split.
+  - intros tid σ.
+    destruct (Hsafe tid σ) as (e2' & σ2 & es & ?).
+    exists e2', σ2, es.
+    apply base_step_prim_step. done.
+  - intros tid σ1 κ e2' σ2 es ?%base_reducible_prim_step.
+    all: eauto using base_reducible_no_obs_base_reducible.
+Qed.
+
+#[global] Instance context_id :
+  Context (@id expr).
+Proof.
+  constructor; naive_solver.
+Qed.
+#[global] Instance context_fill K :
+  Context (fill K).
+Proof.
+  split => /=.
+  - auto using fill_not_val.
+  - intros ? ? ? ? ? ? ? [K' e1' e2' Heq1 Heq2 Hstep].
+    exists (K' ++ K) e1' e2'.
+    all: rewrite ?Heq1 ?Heq2 ?fill_app //.
+  - intros tid e1 σ1 κ e2 σ2 es Hnval [K'' e1'' e2'' Heq1 -> Hstep].
+    destruct (step_by_val tid K K'' e1 e1'' σ1 κ e2'' σ2 es) as [K' ->]; try done.
+    rewrite fill_app in Heq1. apply (inj (fill _)) in Heq1.
+    exists (fill K' e2''). rewrite fill_app. split; first done.
+    eauto using prim_step.
+Qed.
+#[global] Instance context_filli k :
+  Context (filli k).
+Proof.
+  change (Context (fill [k])). apply _.
+Qed.
+
+Lemma reducible_context (K : expr → expr) `{!Context K} tid e σ :
+  reducible tid e σ →
+  reducible tid (K e) σ.
+Proof.
+  rewrite /reducible.
+  naive_solver eauto using context_fill_step.
+Qed.
+Lemma reducible_context_inv (K : expr → expr) `{!Context K} tid e σ :
+  to_val e = None →
+  reducible tid (K e) σ →
+  reducible tid e σ.
+Proof.
+  intros He (e' & σ' & k & es & Hstep). rewrite /reducible.
+  apply context_fill_step_inv in Hstep as (e2' & _ & Hstep); naive_solver.
+Qed.
+
+Lemma pure_step_context (K : expr → expr) `{!Context K} e1 e2 :
+  pure_step e1 e2 →
+  pure_step (K e1) (K e2).
+Proof.
+  intros [Hred Hstep]. split.
+  - rewrite /reducible_no_obs in Hred |- *. naive_solver eauto using context_fill_step.
+  - intros tid σ1 κ e2' σ2 es Hpstep.
+    destruct (context_fill_step_inv tid e1 σ1 κ e2' σ2 es) as (e2'' & -> & ?); [|exact Hpstep|].
+    + destruct (Hred tid σ1) as (? & ? & ? & ?); eauto using prim_step_not_val.
+    + edestruct (Hstep tid σ1 κ e2'' σ2 es) as (? & -> & -> & ->); done.
+Qed.
+Lemma pure_step_nsteps_context (K : expr → expr) `{!Context K} n e1 e2 :
+  relations.nsteps pure_step n e1 e2 →
+  relations.nsteps pure_step n (K e1) (K e2).
+Proof.
+  eauto using nsteps_congruence, pure_step_context.
+Qed.
+
+Lemma pure_exec_context (K : expr → expr) `{!Context K} ϕ n e1 e2 :
+  PureExec ϕ n e1 e2 →
+  PureExec ϕ n (K e1) (K e2).
+Proof.
+  rewrite /PureExec; auto using pure_step_nsteps_context.
+Qed.
+Lemma pure_exec_fill K ϕ n e1 e2 :
+  PureExec ϕ n e1 e2 →
+  PureExec ϕ n (fill K e1) (fill K e2).
+Proof.
+  apply: pure_exec_context.
+Qed.
+
+Lemma sub_redexes_are_values_alt e :
+  ( ∀ k e',
+    e = filli k e' →
+    is_Some (to_val e')
+  ) →
+  sub_redexes_are_values e.
+Proof.
+  intros H K e' ->.
+  destruct K as [| k K _] using rev_ind => //=.
+  intros []%eq_None_not_Some.
+  eapply fill_val, H. rewrite fill_app //.
+Qed.
 
 Lemma to_val_fill_some K e v :
   to_val (fill K e) = Some v →
@@ -58,6 +455,31 @@ Proof.
   intro H. destruct H as [K e1 e2 H1 H2].
   assert (to_val (fill K e2) = Some v) as H3; first rewrite -H2 //.
   apply to_val_fill_some in H3 as [-> ->]. subst e. done.
+Qed.
+
+Lemma silent_steps_nsteps ρ1 ρ2 :
+  rtc silent_step ρ1 ρ2 ↔
+    ∃ n κs,
+    nsteps n ρ1 κs ρ2.
+Proof.
+  rewrite /silent_step. split.
+  - induction 1; naive_solver.
+  - intros (n & κs & Hsteps).
+    induction Hsteps; eauto using rtc.
+Qed.
+
+Lemma step_length ρ1 κ ρ2 :
+  step ρ1 κ ρ2 →
+  length ρ1.1 ≤ length ρ2.1.
+Proof.
+  intros (tid & e1 & e2 & σ2 & es & Hstep & Hlookup & ->).
+  simpl_length/=. lia.
+Qed.
+Lemma nsteps_length n ρ1 κs ρ2 :
+  nsteps n ρ1 κs ρ2 →
+  length ρ1.1 ≤ length ρ2.1.
+Proof.
+  induction 1 as [| ? ? ? ? ? ? Hstep%step_length]; lia.
 Qed.
 
 Lemma base_reducible_no_obs_equal tid v1 v2 σ :
@@ -124,8 +546,8 @@ Proof.
   - invert Hstep.
     constructor. done.
   - rewrite fill_app /= in Hfill. destruct k; inversion Hfill; subst; clear Hfill.
-    + assert (fill_item k (fill K e1') = fill (K ++ [k]) e1') as Heq1; first by rewrite fill_app.
-      assert (fill_item k (fill K e2') = fill (K ++ [k]) e2') as Heq2; first by rewrite fill_app.
+    + assert (filli k (fill K e1') = fill (K ++ [k]) e1') as Heq1; first by rewrite fill_app.
+      assert (filli k (fill K e2') = fill (K ++ [k]) e2') as Heq2; first by rewrite fill_app.
       rewrite fill_app /=. rewrite Heq1 in Hatomic.
       assert (is_Some (to_val (fill (K ++ [k]) e2'))) as H.
       { eapply (Hatomic tid σ1 _ κ σ2 es), (base_step_fill_prim_step' (K ++ [k])); done. }
@@ -138,28 +560,4 @@ Proof.
       assert (to_val (fill K e1') = Some v2) as Hfill_v2 by rewrite -Hv2 //.
       apply to_val_fill_some in Hfill_v2 as (-> & ->).
       invert Hstep.
-Qed.
-
-Lemma irreducible_resolve tid e v1 v2 σ :
-  irreducible tid e σ →
-  irreducible tid (Resolve e (Val v1) (Val v2)) σ.
-Proof.
-  intros H κ ? σ' es [K' e1' e2' Hfill -> step].
-  simplify.
-  induction K' as [| K K' _] using rev_ind; simpl in Hfill.
-  - subst e1'. inversion step. eapply H. apply base_step_prim_step. done.
-  - rewrite fill_app /= in Hfill.
-    destruct K.
-    all: inversion Hfill; subst; clear Hfill.
-    all:
-      try
-        match goal with H: Val ?v = fill _ ?e |- _ =>
-          assert (to_val (fill K' e) = Some v) as Heq by rewrite -H //;
-          apply to_val_fill_some in Heq;
-          destruct Heq as [-> ->];
-          inversion step
-        end.
-    eapply (H κ (fill_item _ (foldl (flip fill_item) e2' K')) σ' es).
-    eapply (base_step_fill_prim_step' (K' ++ [_])); last done.
-    all: rewrite /= fill_app //.
 Qed.
