theories/zoo/program_logic/atomic.v
@@ -1,14 +1,244 @@
-From iris.bi Require Import
-  telescopes.
-
 From zoo Require Import
   prelude.
-From zoo.iris.program_logic Require Export
-  atomic.
+From zoo.iris Require Import
+  diaframe.
+From zoo.iris.bi Require Export
+  lib.atomic.
 From zoo.program_logic Require Export
   wp.
 From zoo Require Import
   options.
+
+Section atomic_acc.
+  Context `{BiFUpd PROP} {TA TB : tele}.
+
+  Implicit Types α : TA → PROP.
+  Implicit Types P : PROP.
+  Implicit Types β Ψ : TA → TB → PROP.
+
+  #[global] Instance atomic_acc_proper Eo Ei :
+    Proper (
+      pointwise_relation TA (≡) ==>
+      (≡) ==>
+      pointwise_relation TA (pointwise_relation TB (≡)) ==>
+      pointwise_relation TA (pointwise_relation TB (≡)) ==>
+      (≡)
+    ) (atomic_acc (PROP := PROP) Eo Ei).
+  Proof.
+    solve_proper.
+  Qed.
+
+  Lemma atomic_acc_frame_l R Eo Ei α P β Ψ :
+    R ∗ atomic_acc Eo Ei α P β Ψ ⊢
+    atomic_acc Eo Ei α (R ∗ P) β (λ.. x y, R ∗ Ψ x y).
+  Proof.
+    iIntros "(HR & H)".
+    iApply (atomic_acc_wand with "[HR] H").
+    iSplit; first iSteps. iIntros "%x %y HΨ". rewrite !tele_app_bind.
+    iSteps.
+  Qed.
+  Lemma atomic_acc_frame_r R Eo Ei α P β Ψ :
+    atomic_acc Eo Ei α P β Ψ ∗ R ⊢
+    atomic_acc Eo Ei α (P ∗ R) β (λ.. x y, Ψ x y ∗ R).
+  Proof.
+    iIntros "(H & HR)".
+    iApply (atomic_acc_wand with "[HR] H").
+    iSplit; first iSteps. iIntros "%x %y HΨ". rewrite !tele_app_bind.
+    iSteps.
+  Qed.
+
+  #[global] Instance frame_atomic_acc p R Eo Ei α P1 P2 β Ψ1 Ψ2 :
+    Frame p R P1 P2 →
+    (∀ x y, Frame p R (Ψ1 x y) (Ψ2 x y)) →
+    Frame p R (atomic_acc Eo Ei α P1 β (λ.. x y, Ψ1 x y)) (atomic_acc Eo Ei α P2 β (λ.. x y, Ψ2 x y)).
+  Proof.
+    rewrite /Frame atomic_acc_frame_l => HR HΨ.
+    iApply atomic_acc_wand. iSplit.
+    - iApply HR.
+    - iIntros "%x %y". rewrite !tele_app_bind.
+      iApply HΨ.
+  Qed.
+
+  #[global] Instance is_except_0_atomic_acc Eo Ei α P β Ψ :
+    IsExcept0 (atomic_acc Eo Ei α P β Ψ).
+  Proof.
+    rewrite /atomic_acc. apply _.
+  Qed.
+End atomic_acc.
+
+Section atomic_update.
+  Context `{BiFUpd PROP} {TA TB : tele}.
+
+  Implicit Types α : TA → PROP.
+  Implicit Types β Ψ : TA → TB → PROP.
+
+  #[global] Instance atomic_update_proper Eo Ei :
+    Proper (
+      pointwise_relation TA (≡) ==>
+      pointwise_relation TA (pointwise_relation TB (≡)) ==>
+      pointwise_relation TA (pointwise_relation TB (≡)) ==>
+      (≡)
+    ) (atomic_update (PROP := PROP) Eo Ei).
+  Proof.
+    rewrite atomic.atomic_update_unseal /atomic.atomic_update_def /atomic_update_pre.
+    solve_proper.
+  Qed.
+
+  Lemma atomic_update_mono Eo Ei α β Ψ1 Ψ2 :
+    (∀.. x y, Ψ1 x y -∗ Ψ2 x y) -∗
+    atomic_update Eo Ei α β Ψ1 -∗
+    atomic_update Eo Ei α β Ψ2.
+  Proof.
+    iIntros "HΨ H".
+    iEval (rewrite atomic.atomic_update_unseal /atomic.atomic_update_def /atomic_update_pre).
+    set Φ := (λ (_ : ()), (∀.. x y, Ψ1 x y -∗ Ψ2 x y) ∗ atomic_update Eo Ei α β Ψ1)%I.
+    iApply (fixpoint_mono.greatest_fixpoint_coiter _ Φ); last iFrame.
+    iIntros "!>" ([]) "(HΨ & H)". rewrite atomic.aupd_unfold /atomic_acc.
+    iMod "H" as "(%x & Hα & H)".
+    iModIntro. iExists x. iFrame. iSplit.
+    - iIntros "Hα". iFrame.
+      iApply ("H" with "Hα").
+    - iIntros "%y Hβ".
+      iMod ("H" with "Hβ") as "HΨ1".
+      iApply "HΨ".
+      iSteps.
+  Qed.
+  Lemma atomic_update_wand Eo Ei α β Ψ1 Ψ2 :
+    atomic_update Eo Ei α β Ψ1 -∗
+    (∀.. x y, Ψ1 x y -∗ Ψ2 x y) -∗
+    atomic_update Eo Ei α β Ψ2.
+  Proof.
+    iIntros "H HΨ".
+    iApply (atomic_update_mono with "HΨ H").
+  Qed.
+
+  Lemma atomic_update_frame_l R Eo Ei α β Ψ :
+    R ∗ atomic_update Eo Ei α β Ψ ⊢
+    atomic_update Eo Ei α β (λ.. x y, R ∗ Ψ x y).
+  Proof.
+    iIntros "(HR & H)".
+    iApply (atomic_update_wand with "H"). iIntros "%x %y HΨ". rewrite !tele_app_bind.
+    iSteps.
+  Qed.
+  Lemma atomic_update_frame_r R Eo Ei α β Ψ :
+    atomic_update Eo Ei α β Ψ ∗ R ⊢
+    atomic_update Eo Ei α β (λ.. x y, Ψ x y ∗ R).
+  Proof.
+    iIntros "(H & HR)".
+    iApply (atomic_update_wand with "H"). iIntros "%x %y HΨ". rewrite !tele_app_bind.
+    iSteps.
+  Qed.
+
+  #[global] Instance frame_atomic_update p R Eo Ei α β Ψ1 Ψ2 :
+    (∀ x y, Frame p R (Ψ1 x y) (Ψ2 x y)) →
+    Frame p R (atomic_update Eo Ei α β (λ.. x y, Ψ1 x y)) (atomic_update Eo Ei α β (λ.. x y, Ψ2 x y)).
+  Proof.
+    rewrite /Frame atomic_update_frame_l => HΨ.
+    iApply atomic_update_mono. iIntros "%x %y". rewrite !tele_app_bind.
+    iApply HΨ.
+  Qed.
+
+  #[global] Instance is_except_0_atomic_update Eo Ei α β Ψ :
+    IsExcept0 (atomic_update Eo Ei α β Ψ).
+  Proof.
+    rewrite /IsExcept0 atomic.aupd_unfold is_except_0 //.
+  Qed.
+End atomic_update.
+
+Section atomic_triple.
+  Context `{zoo_G : !ZooG Σ} {TA TB TP : tele}.
+
+  Implicit Types P : iProp Σ.
+  Implicit Types α : TA → iProp Σ.
+  Implicit Types β : TA → TB → iProp Σ.
+  Implicit Types Ψ : TA → TB → TP → iProp Σ.
+  Implicit Types f : TA → TB → TP → val.
+
+  Definition atomic_triple e tid E P α β Ψ f : iProp Σ :=
+    ∀ Φ,
+    P -∗
+    atomic_update (⊤ ∖ E) ∅ α β (λ.. x y, ∀.. z, Ψ x y z -∗ Φ (f x y z)) -∗
+    WP e ∷ tid {{ Φ }}.
+  #[global] Arguments atomic_triple e%_E tid E (P α β Ψ f)%_I : assert.
+
+  #[global] Instance atomic_triple_ne e tid E n :
+    Proper (
+      (≡{n}≡) ==>
+      pointwise_relation TA (≡{n}≡) ==>
+      pointwise_relation TA (pointwise_relation TB (≡{n}≡)) ==>
+      pointwise_relation TA (pointwise_relation TB (pointwise_relation TP (≡{n}≡))) ==>
+      pointwise_relation TA (pointwise_relation TB (pointwise_relation TP (=))) ==>
+      (≡{n}≡)
+    ) (atomic_triple e tid E).
+  Proof.
+    rewrite /atomic_triple => P1 P2 HP α1 α2 Hα β1 β2 Hβ Ψ1 Ψ2 HΨ f1 f2 Hf.
+    do 3 f_equiv; first done.
+    do 2 f_equiv; [done.. |].
+    intros x y. rewrite !tele_app_bind.
+    do 3 f_equiv; first apply HΨ.
+    f_equiv. apply Hf.
+  Qed.
+  #[global] Instance atomic_triple_proper e tid E :
+    Proper (
+      (≡) ==>
+      pointwise_relation TA (≡) ==>
+      pointwise_relation TA (pointwise_relation TB (≡)) ==>
+      pointwise_relation TA (pointwise_relation TB (pointwise_relation TP (≡))) ==>
+      pointwise_relation TA (pointwise_relation TB (pointwise_relation TP (=))) ==>
+      (≡)
+    ) (atomic_triple e tid E).
+  Proof.
+    rewrite /atomic_triple => P1 P2 HP α1 α2 Hα β1 β2 Hβ Ψ1 Ψ2 HΨ f1 f2 Hf.
+    do 3 f_equiv; first done.
+    do 2 f_equiv; [done.. |].
+    intros x y. rewrite !tele_app_bind.
+    do 3 f_equiv; first apply HΨ.
+    f_equiv. apply Hf.
+  Qed.
+
+  Lemma atomic_triple_mono e tid E P α β Ψ1 Ψ2 f :
+    (∀.. x y z, Ψ1 x y z -∗ Ψ2 x y z) -∗
+    atomic_triple e tid E P α β Ψ1 f -∗
+    atomic_triple e tid E P α β Ψ2 f.
+  Proof.
+    iIntros "HΨ H %Φ HP HΦ".
+    iApply ("H" with "HP").
+    iApply (atomic_update_wand with "HΦ"). iIntros "%x %y HΨ2". rewrite !tele_app_bind. iIntros "%z HΨ1".
+    iApply "HΨ2".
+    iApply "HΨ".
+    iSteps.
+  Qed.
+  Lemma atomic_triple_wand e tid E P α β Ψ1 Ψ2 f :
+    atomic_triple e tid E P α β Ψ1 f -∗
+    (∀.. x y z, Ψ1 x y z -∗ Ψ2 x y z) -∗
+    atomic_triple e tid E P α β Ψ2 f.
+  Proof.
+    iIntros "H HΨ".
+    iApply (atomic_triple_mono with "HΨ H").
+  Qed.
+
+  #[global] Instance frame_atomic_triple p R e tid E P α β Ψ1 Ψ2 f :
+    (∀ x y z, Frame p R (Ψ1 x y z) (Ψ2 x y z)) →
+    Frame p R (atomic_triple e tid E P α β (λ.. x y, Ψ1 x y) f) (atomic_triple e tid E P α β (λ.. x y, Ψ2 x y) f).
+  Proof.
+    iIntros "/= %HΨ (HR & H)".
+    iApply (atomic_triple_wand with "H"). iIntros "%x %y %z HΨ2". rewrite !tele_app_bind.
+    iApply HΨ.
+    iSteps.
+  Qed.
+End atomic_triple.
+
+Declare Custom Entry atomic_triple_mask.
+Notation "" := (
+  @empty coPset _
+)(in custom atomic_triple_mask
+).
+Notation "@ E" :=
+  E
+( in custom atomic_triple_mask at level 200,
+  E constr,
+  format "'/  ' @  E "
+).
 
 Notation "'<<<' P | ∀∀ x1 .. xn , α '>>>' e tid E '<<<' ∃∃ y1 .. yn , β | z1 .. zn , 'RET' v ; Q '>>>'" := (
   atomic_triple
