theories/zoo/program_logic/wp_adequacy.v
@@ -1,0 +1,46 @@
+From zoo Require Import
+  prelude.
+From zoo.iris Require Import
+  diaframe.
+From zoo.program_logic Require Export
+  bwp_adequacy
+  wp.
+From zoo Require Import
+  options.
+
+Implicit Types e : expr.
+Implicit Types v : val.
+Implicit Types σ : state.
+
+Lemma wp_adequacy' `{inv_Gpre : !invGpreS Σ} e σ :
+  ( ∀ `{inv_G : !invGS Σ} κs,
+    ⊢ |={⊤}=>
+      ∃ (zoo_G : ZooG Σ) Φ,
+      ⌜zoo_G.(zoo_G_inv_G) = inv_G⌝ ∗
+      state_interp 1 σ κs ∗
+      WP e ∶ 0 {{ Φ }}
+  ) →
+  safe ([e], σ).
+Proof.
+  intros H.
+  apply: bwp_adequacy' => inv_G κs.
+  iMod H as "(%zoo_G & %Φ & <- & Hinterp & Hwp)".
+  iExists zoo_G, Φ. iFrameSteps.
+  iApply (wp_bwp with "Hwp").
+Qed.
+Lemma wp_adequacy `{zoo_Gpre : !ZooGpre Σ} {e σ} param :
+  state_wf σ param →
+  ( ∀ `{zoo_G : !ZooG Σ},
+    ⊢ ∃ Φ,
+      ([∗ map] l ↦ v ∈ state_heap_initial σ, l ↦ v) -∗
+      0 ↦ₗ param.(zoo_parameter_local) -∗
+      WP e ∶ 0 {{ Φ }}
+  ) →
+  safe ([e], σ).
+Proof.
+  intros Hwf Hwp.
+  apply: wp_adequacy' => // Hinv_G κs.
+  iMod (zoo_init σ param κs) as "(%zoo_G & <- & Hinterp & Hheap & Hlocals)"; first done.
+  iDestruct (Hwp zoo_G) as "(%Φ & Hwp)".
+  iExists zoo_G, Φ. iFrameSteps.
+Qed.
